KHeap_A lemmas done

proof/invariant-abstract/New.thy
@@ -1,21 +1,21 @@
 theory New
-imports
-  KernelInit_AI
- "$L4V_ARCH/ArchDetSchedSchedule_AI"
+  imports
+    KernelInit_AI
+    "$L4V_ARCH/ArchDetSchedSchedule_AI"
 begin
-(*declare [[show_types]]*)
+  (*declare [[show_types]]*)
 axiomatization
   colour_oracle :: "domain \<Rightarrow> obj_ref set"
-where
-  colour_oracle_no_overlap: "x \<noteq> y \<longrightarrow> (colour_oracle x \<inter> colour_oracle y = {})"
+  where
+    colour_oracle_no_overlap: "x \<noteq> y \<longrightarrow> (colour_oracle x \<inter> colour_oracle y = {})"
 
 term "obj_refs"
 term "obj_ref_of"
 
 definition
   check_cap_ref :: "cap \<Rightarrow> obj_ref set \<Rightarrow> bool"
-where
-  "check_cap_ref cap obj_set \<equiv> obj_refs cap \<subseteq> obj_set"
+  where
+    "check_cap_ref cap obj_set \<equiv> obj_refs cap \<subseteq> obj_set"
 
 
 term "ArchInvariants_AI.RISCV64.obj_addrs" (* should be used everywhere? *)
@@ -25,12 +25,12 @@ term "obj_addrs"
 
 primrec
   check_kernel_object_ref :: "kernel_object \<Rightarrow> obj_ref set \<Rightarrow> bool"
-where
-  "check_kernel_object_ref (CNode _ cs) obj_dom =
+  where
+    "check_kernel_object_ref (CNode _ cs) obj_dom =
     (\<forall>x.
       case (cs x) of Some cap \<Rightarrow> check_cap_ref cap obj_dom
                    | None \<Rightarrow> True)"
-| "check_kernel_object_ref (TCB t) obj_dom =
+  | "check_kernel_object_ref (TCB t) obj_dom =
     (check_cap_ref (tcb_ctable t) obj_dom \<and>
     check_cap_ref (tcb_vtable t) obj_dom \<and>
     check_cap_ref (tcb_reply t) obj_dom \<and>
@@ -42,15 +42,15 @@ where
                          | _ \<Rightarrow> True) \<and>
     tcb_ipc_buffer t \<in> obj_dom \<and>
     set_option (tcb_bound_notification t) \<subseteq> obj_dom)"
-| "check_kernel_object_ref (Endpoint ep) obj_dom = (case ep of IdleEP \<Rightarrow> True
+  | "check_kernel_object_ref (Endpoint ep) obj_dom = (case ep of IdleEP \<Rightarrow> True
                                                              | SendEP s \<Rightarrow> (set s \<subseteq> obj_dom)
                                                              | RecvEP r \<Rightarrow>  (set r \<subseteq> obj_dom))"
-| "check_kernel_object_ref (Notification ntfn) obj_dom =
+  | "check_kernel_object_ref (Notification ntfn) obj_dom =
     ((case (ntfn_obj ntfn) of WaitingNtfn l \<Rightarrow> set l \<subseteq> obj_dom
                             | _ \<Rightarrow> True)
     \<and> (case (ntfn_bound_tcb ntfn) of Some tcb \<Rightarrow> tcb \<in> obj_dom
                                    | None \<Rightarrow> True))"
-| "check_kernel_object_ref (ArchObj ao) obj_dom = (case ao of RISCV64_A.DataPage _ _ \<Rightarrow> True
+  | "check_kernel_object_ref (ArchObj ao) obj_dom = (case ao of RISCV64_A.DataPage _ _ \<Rightarrow> True
                                                             | RISCV64_A.ASIDPool ap \<Rightarrow> (\<forall>x.
                                                                 case (ap x) of Some obj_ref \<Rightarrow> obj_ref \<in> obj_dom
                                                                              | None \<Rightarrow> True)
@@ -60,91 +60,77 @@ where
                                                                              | RISCV64_A.PageTablePTE ppn _  \<Rightarrow> RISCV64_A.addr_from_ppn ppn \<in> obj_dom))"
 
 definition colour_invariant
-where
-  "colour_invariant s \<equiv> \<forall>ptr kobj. (ko_at kobj ptr s \<and> ptr \<in> colour_oracle (cur_domain s)) \<longrightarrow> check_kernel_object_ref kobj (colour_oracle (cur_domain s))"
+  where
+    "colour_invariant s \<equiv> \<forall>ptr kobj.
+    (ko_at kobj ptr s \<and> ptr \<in> colour_oracle (cur_domain s)) \<longrightarrow>
+    check_kernel_object_ref kobj (colour_oracle (cur_domain s))"
 
 lemma set_object_colour_maintained:
   "\<lbrace>colour_invariant and (\<lambda>s. check_kernel_object_ref kobj (colour_oracle (cur_domain s)))\<rbrace>
    set_object ptr kobj
    \<lbrace>\<lambda>_. colour_invariant\<rbrace>"
-apply (wp add: set_object_wp)
-apply (simp add: colour_invariant_def)
-apply wpsimp
-apply (simp add: obj_at_update)
+  apply (wp add: set_object_wp)
+  apply (simp add: colour_invariant_def)
+  apply wpsimp
+  apply (simp add: obj_at_update)
   by presburger
 
 lemma thread_set_colour_maintained:
   "\<lbrace>colour_invariant and (\<lambda>s. let tcb = TCB (f $ the (get_tcb ptr s)) in check_kernel_object_ref tcb (colour_oracle (cur_domain s)))\<rbrace>
    thread_set f ptr
   \<lbrace>\<lambda>_. colour_invariant\<rbrace>"
-apply (wp add: thread_set_wp)
-apply (simp add: colour_invariant_def)
-apply (simp add: obj_at_update)
-by fastforce
+  apply (wp add: thread_set_wp)
+  apply (simp add: colour_invariant_def)
+  apply (simp add: obj_at_update)
+  by fastforce
 
 lemma thread_set_priority_colour_maintained:
   "\<lbrace>colour_invariant\<rbrace>
-   thread_set_priority ptr prio
-  \<lbrace>\<lambda>_. colour_invariant\<rbrace>"
+     thread_set_priority ptr prio
+    \<lbrace>\<lambda>_. colour_invariant\<rbrace>"
   apply (simp add: thread_set_priority_def)
   apply (wp add: thread_set_wp)
   apply (simp add: colour_invariant_def obj_at_update)
-apply (rule allI)
-apply (rule impI)
-apply (rule impI)
-apply auto
-by fastforce+
+  by fastforce+
 
 lemma thread_set_time_slice_colour_maintained:
   "\<lbrace>colour_invariant\<rbrace>
-   thread_set_time_slice ptr prio
-  \<lbrace>\<lambda>_. colour_invariant\<rbrace>"
+     thread_set_time_slice ptr prio
+    \<lbrace>\<lambda>_. colour_invariant\<rbrace>"
   apply (simp add: thread_set_time_slice_def)
   apply (wp add: thread_set_wp)
   apply (simp add: colour_invariant_def obj_at_update)
-apply (rule allI)
-apply (rule impI)
-apply (rule impI)
-apply auto
-by fastforce+
+  by fastforce+
 
 lemma thread_set_domain_colour_maintained:
   "\<lbrace>colour_invariant\<rbrace>
-   thread_set_domain ptr prio
-  \<lbrace>\<lambda>_. colour_invariant\<rbrace>"
+     thread_set_domain ptr prio
+    \<lbrace>\<lambda>_. colour_invariant\<rbrace>"
   apply (simp add: thread_set_domain_def)
   apply (wp add: thread_set_wp)
   apply (simp add: colour_invariant_def obj_at_update)
-apply (rule allI)
-apply (rule impI)
-apply (rule impI)
-apply auto
-by fastforce+
+  by fastforce+
 
 lemma set_mcpriority_colour_maintained:
   "\<lbrace>colour_invariant\<rbrace>
-   set_mcpriority ref mcp
-  \<lbrace>\<lambda>_. colour_invariant\<rbrace>"
+     set_mcpriority ref mcp
+    \<lbrace>\<lambda>_. colour_invariant\<rbrace>"
   apply (simp add: set_mcpriority_def)
   apply (wp add: thread_set_wp)
   apply (simp add: colour_invariant_def obj_at_update)
-apply (rule allI)
-apply (rule impI)
-apply (rule impI)
-apply auto
-by fastforce+
+  by fastforce+
 
 lemma arch_thread_set_colour_maintained:
   "\<lbrace>colour_invariant and (\<lambda>s.
-      let tcb = the $ get_tcb ptr s in
-      let arch_tcb = f $ tcb_arch tcb in
-      let new_tcb = TCB $ tcb \<lparr> tcb_arch := arch_tcb \<rparr> in
-      check_kernel_object_ref new_tcb (colour_oracle (cur_domain s)))\<rbrace>
-   arch_thread_set f ptr
-  \<lbrace>\<lambda>_. colour_invariant\<rbrace>"
-apply (wp add: arch_thread_set_wp)
-apply (simp add: colour_invariant_def)
-apply (simp add: obj_at_update)
+        let tcb = the $ get_tcb ptr s in
+        let arch_tcb = f $ tcb_arch tcb in
+        let new_tcb = TCB $ tcb \<lparr> tcb_arch := arch_tcb \<rparr> in
+        check_kernel_object_ref new_tcb (colour_oracle (cur_domain s)))\<rbrace>
+     arch_thread_set f ptr
+    \<lbrace>\<lambda>_. colour_invariant\<rbrace>"
+  apply (wp add: arch_thread_set_wp)
+  apply (simp add: colour_invariant_def)
+  apply (simp add: obj_at_update)
   by fastforce
 
 lemma set_bound_notification_colour_maintained:
@@ -154,104 +140,78 @@ lemma set_bound_notification_colour_maintained:
   apply (simp add: set_bound_notification_thread_set)
   apply (wp add: thread_set_wp)
   apply (simp add: colour_invariant_def obj_at_update)
-apply (rule allI)
-apply (rule impI)
-apply (rule impI)
-apply auto
-by fastforce+
+  by fastforce+
 
 lemma set_simple_ko_colour_maintained:
   "\<lbrace>colour_invariant and (\<lambda>s.
-      let kobj = f ep in
-        ko_at kobj ptr s \<longrightarrow>
-        is_simple_type kobj \<longrightarrow>
-        partial_inv f kobj \<noteq> None \<longrightarrow>
-        check_kernel_object_ref (f ep) (colour_oracle (cur_domain s)))\<rbrace>
-   set_simple_ko f ptr ep
-  \<lbrace>\<lambda>_. colour_invariant\<rbrace>"
-(*apply (wpsimp simp: get_simple_ko_def partial_inv_def the_equality split: kernel_object.splits)*)
-apply (unfold set_simple_ko_def)
-apply wpsimp
-apply (wp add: get_object_wp set_object_wp)+
-apply (rule allI)
-apply (rule impI)+
-apply (simp add: obj_at_update colour_invariant_def)
-apply (rule allI)+
-apply (rule impI)
-apply wpsimp
-apply (simp add: Let_def split: if_splits)
-apply (rename_tac out_s out_ko out_ptra out_kobj out_y)
-apply (unfold obj_at_def)
-apply clarsimp
-apply (case_tac "out_ptra = ptr")
-(*apply clarsimp (* looks like it removes a necessary assumption? *)*)
-apply simp
-apply (erule disjE)
-apply clarsimp
-apply (erule allE)+
-apply (erule impE)+
-apply (rule conjI)
-sorry
-
-find_theorems "ko_at"
-find_theorems "a_type"
-find_theorems "set_simple_ko"
-
-(*apply (simp only: fun_upd_apply[symmetric])*)
-lemma tmp_colour_maintained:
-  "\<lbrace>colour_invariant and (\<lambda>s.
-      \<lbrace>colour_invariant\<rbrace>
-      f
-      \<lbrace>\<lambda>rv s.
-          \<forall>ptr kobj.
-             ko_at kobj ptr s \<and>
-             ptr
-             \<in> colour_oracle (cur_domain s) \<longrightarrow>
-             check_kernel_object_ref kobj
-              (colour_oracle (cur_domain s))\<rbrace>)\<rbrace>
-    throw_on_false ex f
+        let kobj = the $ kheap s ptr in
+          is_simple_type kobj \<longrightarrow>
+          partial_inv f kobj \<noteq> None \<longrightarrow>
+          check_kernel_object_ref (f ep) (colour_oracle (cur_domain s)))\<rbrace>
+     set_simple_ko f ptr ep
     \<lbrace>\<lambda>_. colour_invariant\<rbrace>"
-sorry
+  apply (unfold set_simple_ko_def)
+  apply wpsimp
+      apply (wp add: get_object_wp set_object_wp)+
+  apply (simp add: obj_at_update colour_invariant_def obj_at_def)
+  by auto
 
-crunch reschedule_required,
-       possible_switch_to,
-       set_thread_state_act,
-       set_priority,
-       set_scheduler_action,
-       tcb_sched_action,
-       set_tcb_queue,
-       set_irq_state for colour_maintained: "colour_invariant"
-  (simp: colour_invariant_def obj_at_update)
+lemma throw_on_false_colour_maintained:
+  "\<lbrace>colour_invariant\<rbrace>
+      f
+    \<lbrace>\<lambda>_ . colour_invariant\<rbrace>
+   \<Longrightarrow>
+   \<lbrace>colour_invariant\<rbrace>
+      throw_on_false ex f
+   \<lbrace>\<lambda>_. colour_invariant\<rbrace>"
+by (simp add: hoare_wp_splits(12)
+    throw_on_false_wp)
 
 lemma set_thread_state_colour_maintained:
   "\<lbrace>colour_invariant and (\<lambda>s.
-      let new_tcb = TCB (tcb \<lparr> tcb_state := ts \<rparr>) in
-      check_kernel_object_ref new_tcb (colour_oracle (cur_domain s)))\<rbrace>
-   set_thread_state ref ts
-  \<lbrace>\<lambda>_. colour_invariant\<rbrace>"
-apply (unfold set_thread_state_def Let_def)
-apply wp
-apply wpsimp
-apply (unfold set_thread_state_act_def set_scheduler_action_def get_thread_state_def)
-apply wpsimp
-apply (wp add: thread_get_wp)
-apply (wp add: set_object_wp)
-apply (wp add: gets_the_wp)
-apply (simp add: obj_at_update)
-apply (unfold colour_invariant_def)
-apply auto
-apply (erule allE)+
-sorry
+        let new_tcb = TCB (tcb \<lparr> tcb_state := ts \<rparr>) in
+        check_kernel_object_ref new_tcb (colour_oracle (cur_domain s)))\<rbrace>
+     set_thread_state ref ts
+    \<lbrace>\<lambda>_. colour_invariant\<rbrace>"
+  apply (unfold set_thread_state_def Let_def)
+  apply wp
+     apply wpsimp
+     apply (unfold set_thread_state_act_def set_scheduler_action_def get_thread_state_def)
+     apply wpsimp
+     apply (wp add: thread_get_wp)
+    apply (wp add: set_object_wp)
+   apply (wp add: gets_the_wp)
+  apply (simp add: obj_at_update obj_at_def)
+  unfolding colour_invariant_def
+  apply (simp add: obj_at_update obj_at_def)
+  by (smt (verit, best) RISCV64.ko_at_kheap
+      check_kernel_object_ref.simps(2)
+      get_tcb_obj_atE option.sel)
 
 lemma as_user_colour_maintained:
   "\<lbrace>colour_invariant\<rbrace>
-   as_user ptr f
-  \<lbrace>\<lambda>_. colour_invariant\<rbrace>"
-apply (unfold as_user_def)
-apply wpsimp
-apply (wp add: set_object_wp)+
-apply auto
-sorry
+     as_user ptr f
+    \<lbrace>\<lambda>_. colour_invariant\<rbrace>"
+  apply (unfold as_user_def)
+  apply wpsimp
+       apply (wp add: set_object_wp)+
+  apply auto
+  unfolding colour_invariant_def
+  apply (simp add: obj_at_update)
+  apply auto
+  apply (case_tac "ptr\<noteq>ptra")
+  apply (simp add: obj_at_def)+
+  using get_tcb_SomeD by fastforce
+
+crunch reschedule_required,
+  possible_switch_to,
+  set_thread_state_act,
+  set_priority,
+  set_scheduler_action,
+  tcb_sched_action,
+  set_tcb_queue,
+  set_irq_state for colour_maintained: "colour_invariant"
+  (simp: colour_invariant_def obj_at_update)
 
 (*crunch thread_set_domain, thread_set_time_slice, thread_set_priority for colour_maintained: "colour_invariant"
   (wp: thread_set_wp
